src/named/Tactics.v
@@ -21,6 +21,22 @@ Ltac2 in_goal id := Fresh.fresh (of_goal ()) id.
 
 Ltac2 fresh s := in_goal (Option.get (Ident.of_string s)).
 
+
+(* taken from https://github.com/coq/coq/issues/11641 *)
+Ltac2 my_change2 (a : constr) (b : constr) :=
+  ltac1:( a b |- change a with b ) (Ltac1.of_constr a) (Ltac1.of_constr b).
+
+
+Ltac2 all_red_flags :=
+  { Std.rBeta := true;
+  Std.rMatch := true;
+  Std.rFix := true;
+  Std.rCofix := true;
+  Std.rZeta := true;
+  Std.rDelta := true;
+  Std.rConst := []
+}.
+
 (*
 tests whether two terms are equal,
 unifying evars as necessary.
@@ -34,17 +50,24 @@ Ltac2 eequal a b :=
        assert ($a = $b)>[solve[f_equal; eauto]|]; true)
     (fun _ => false).
 
+Ltac2 change_cbv e :=
+  my_change2 e (Std.eval_cbv all_red_flags e).
+
 (* Attempts to clear a goal of the form
    'a \in l', unifying evars as necessary *)
+Ltac2 Type exn ::= [UnifyInFailure].
 Ltac2 rec unify_in () :=
-  match! goal with
-    [|- is_true (?r \in ?r'::?l)] =>
-    rewrite in_cons;
-    ltac1:(apply /orP);
-    match eequal r r' with
-    | true => left;ltac1:(by apply /eqP)
-    | false => right; unify_in()
-    end
+  lazy_match! goal with
+   | [|- is_true (?r \in ?r'::?l)] =>
+      change_cbv r;
+      rewrite in_cons;
+      ltac1:(apply /orP);
+      match eequal r r' with
+      | true => left;ltac1:(by apply /eqP)
+      | false => right; unify_in()
+      end
+   | [|- is_true (_ \in [::])] => Control.zero UnifyInFailure
+   | [|- is_true (_ \in ?l)] => change_cbv l; unify_in ()
   end.
 
 Require Import String.
@@ -53,15 +76,6 @@ Ltac2 try f :=
   Control.enter
     (fun () => Control.plus f (fun _ => ())).
 
-Ltac2 all_red_flags :=
-  { Std.rBeta := true;
-  Std.rMatch := true;
-  Std.rFix := true;
-  Std.rCofix := true;
-  Std.rZeta := true;
-  Std.rDelta := true;
-  Std.rConst := []
-}.
 
 Ltac2 goal_lang () :=
   lazy_match! goal with
@@ -75,72 +89,12 @@ end.
 
 
 
-(* taken from https://github.com/coq/coq/issues/11641 *)
-Ltac2 my_change2 (a : constr) (b : constr) :=
-  ltac1:( a b |- change a with b ) (Ltac1.of_constr a) (Ltac1.of_constr b).
 
 Ltac2 unify_eq () :=
   match! goal with
     [|- ?a = ?b] =>
     solve[f_equal; eauto]
   end.
-
-Ltac2 Type exn ::= [JudgmentMismatchExn(constr, constr)].
-Ltac2 apply_rule (name : constr) :=
-  let l := goal_lang () in
-  (* TODO: make d an evar so it isn't silently returned?*)
-  let d := constr:(sort_rule [::]) in
-  let r := Std.eval_cbv all_red_flags
-           constr:(named_list_lookup $d $l $name) in
-  lazy_match! r with
-  | sort_rule ?c' =>
-    lazy_match! goal with
-    | [|- wf_sort ?l ?c ?t] =>
-      eapply (@wf_sort_by $l $c $name) >
-      [ unify_in ()|]
-    | [|- ?j] =>
-      Control.zero
-        (JudgmentMismatchExn constr:(($name,$r)) j)
-    end
-  | term_rule ?c' ?t' =>
-    lazy_match! goal with
-    | [|- wf_term ?l ?c ?e ?t] =>
-      ltac1:(l c e t t'|-
-             let s := fresh "s" in
-             evar (s : subst);
-             replace (wf_term l c e t) with
-                (wf_term l c e t'[/s/]);
-            unfold s;
-            clear s
-            ) (Ltac1.of_constr l)
-              (Ltac1.of_constr c)
-              (Ltac1.of_constr e)
-              (Ltac1.of_constr t)
-              (Ltac1.of_constr t') >
-            [ eapply (@wf_term_by $l $c $name) >
-              [ unify_in () |]
-            | unify_eq()]
-    | [|- ?j] =>
-      Control.zero
-        (JudgmentMismatchExn constr:(($name,$r)) j)
-    end
-end.
-
-Check wf_sort_by.
-Goal wf_term [:: [:| |- "foo" : #"bar"]] [::] (con "foo" [::])
-(srt "bar" [::]).
-Proof.
-  
-  apply_rule constr:("foo"%string).
-  
-  admit.
-  cbv.
-  unfold substable_sort.
-  f_equal; eauto.
-  unify_eq ().
-  
-TODO: deconstruct subst automatically based on c'  
-  
 
 (* TODO: generalize over key, value types? *)
 Ltac2 Type rec FinMap :=
@@ -185,23 +139,17 @@ Ltac2 rec map_merge m1 m2 :=
 
 Ltac2 Type exn ::= [DomainExn(constr, constr, constr)].
 Ltac2 dom_exn c t := DomainExn c (Constr.type c) t.
-(* TODO: do this for coq strings*)
-Ltac2 rec int_of_nat c :=
-  match! c with
-  | 0 => 0
-  | S ?c' => Int.add 1 (int_of_nat c')
-  | _ => Control.throw (dom_exn c constr:(nat)) 
-  end.
 
 Ltac2 Type exn ::= [ExpMatchExn(constr, constr)].
 Ltac2 rec exp_match (p : constr) e :=
-  match! p with
-  | var ?x => MapCons (int_of_nat x) e MapEmpty
+  lazy_match! p with
+  | var ?x => MapCons x e MapEmpty
   | con ?pn ?ps =>
-    match! e with
+    (* TODO: handle when e is an existential *)
+    lazy_match! e with
     | con ?n ?s =>
       match Constr.equal pn n with
-      | true => subst_match ps s
+      | true => exp_list_match ps s
       | false => Control.throw (ExpMatchExn p e)
       end
     | var _ => Control.throw (ExpMatchExn p e)
@@ -210,16 +158,128 @@ Ltac2 rec exp_match (p : constr) e :=
     end
   | _ => Control.throw (dom_exn p constr:(exp))
   end
-with subst_match p s :=
-    match! p with
-    | [::] => match! s with [::] => MapEmpty end
+with exp_list_match p s :=
+    lazy_match! p with
+    | [::] => lazy_match! s with [::] => MapEmpty end
     | ?pe::?p' =>
-      match! s with
+      lazy_match! s with
       | ?e::?s' =>
-        map_merge (exp_match pe e) (subst_match p' s')
+        map_merge (exp_match pe e) (exp_list_match p' s')
       | [::] => Control.throw (ExpMatchExn p s)
       end
-    end.
+end.
+
+Ltac2 sort_match p e :=
+  lazy_match! p with
+  | srt ?pn ?ps =>
+    (* TODO: handle when e is an existential *)
+    lazy_match! e with
+    | srt ?n ?s =>
+      match Constr.equal pn n with
+      | true => exp_list_match ps s
+      | false => Control.throw (ExpMatchExn p e)
+      end
+    | var _ => Control.throw (ExpMatchExn p e)
+    | _ => Control.throw (dom_exn e constr:(exp))
+      (* TODO: need to handle evars*)
+    end
+  | _ => Control.throw (dom_exn p constr:(exp))
+  end.
+  
+
+(* Convert a map into a substition constr
+   according to its output ctx constr *)
+Ltac2 rec subst_of_map m c :=
+  lazy_match! c with
+  | [::] => constr:([::])
+  | (?n,_)::?c' =>
+    let v := map_lookup n m in
+    let tl := subst_of_map m c' in
+    constr:(($n,$v)::$tl)
+  end.
+
+Ltac2 Type exn ::= [JudgmentMismatchExn(constr, constr)].
+Ltac2 apply_rule (name : constr) :=
+  let l := goal_lang () in
+  (* TODO: make d an evar so it isn't silently returned?*)
+  let d := constr:(sort_rule [::]) in
+  let r := Std.eval_cbv all_red_flags
+           constr:(named_list_lookup $d $l $name) in
+  lazy_match! r with
+  | sort_rule ?c' =>
+    lazy_match! goal with
+    | [|- wf_sort ?l ?c ?t] =>
+      eapply (@wf_sort_by $l $c $name) >
+      [ unify_in ()|]
+    | [|- ?j] =>
+      Control.zero
+        (JudgmentMismatchExn constr:(($name,$r)) j)
+    end
+  | term_rule ?c' ?t' =>
+    lazy_match! goal with
+    | [|- wf_term ?l ?c ?e ?t] =>
+      ltac1:(l c e t t'|-
+             let s := fresh "s" in
+             evar (s : subst);
+             replace (wf_term l c e t) with
+                (wf_term l c e t'[/s/]);
+            unfold s;
+            clear s
+            ) (Ltac1.of_constr l)
+              (Ltac1.of_constr c)
+              (Ltac1.of_constr e)
+              (Ltac1.of_constr t)
+              (Ltac1.of_constr t') >
+            [ eapply (@wf_term_by $l $c $name) >
+              [ unify_in () |]
+            | unify_eq()]
+    | [|- ?j] =>
+      Control.zero
+        (JudgmentMismatchExn constr:(($name,$r)) j)
+    end
+  | sort_le ?c' ?t1' ?t2' =>
+    lazy_match! goal with
+    | [|- le_sort ?l ?c ?t1 ?t2] =>
+      let m := map_merge
+                 (sort_match t1' t1)
+                 (sort_match t2' t2) in
+      let s := subst_of_map m c' in
+      my_change2
+        '(le_sort $l $c $t1 $t2)
+        '(le_sort $l $c $t1'[/$s/] $t2'[/$s/]);
+      eapply le_sort_subst;
+      Control.enter
+        (fun () =>
+           match! goal with
+           | [|- le_sort _ _ _ _] =>
+             eapply le_sort_by;
+             unify_in ()
+           | [|- le_subst _ _ _ _ _] => ()
+           | [|- _] => Control.throw Match_failure
+           end)
+    | [|- ?j] =>
+      Control.zero
+        (JudgmentMismatchExn constr:(($name,$r)) j)
+    end
+      
+end.
+(* TODO:
+Check wf_sort_by.
+Goal le_sort [:: [s> |-("req") #"foo" = #"bar"]] [::] (srt "foo" [::])
+(srt "bar" [::]).
+Proof.
+  
+  apply_rule constr:("req"%string).
+  
+  admit.
+  cbv.
+  unfold substable_sort.
+  f_equal; eauto.
+  unify_eq ().
+  
+TODO: deconstruct subst automatically based on c'  
+
+
 
 Ltac2 Eval (exp_match constr:(var 1) constr:(var 2)).
 Ltac2 Eval
@@ -297,3 +357,4 @@ Ltac2 apply_term_rule n :=
 end.
 
 
+*)
